src/Pyrosome/Lang/Pi.v
@@ -6,8 +6,8 @@ From Utils Require Import Utils.
 From Pyrosome Require Import
   Theory.Core Elab.Elab
   Elab.PreRule
-  Tools.Matches Tools.EGraph.TypeInference
-  Tools.EGraph.ComputeWf
+  Tools.Resolution Tools.EGraph.ComputeWf
+  Tools.EGraph.TypeInference
   Tools.Interactive
   Lang.Subst
   Lang.SubstEqnGen.
@@ -16,45 +16,6 @@ Require Coq.derive.Derive.
 
 Import Core.Notations.
 Import PreRule.Notations.
-
-
-Import Tools.ComputeWf.
-
-(*TODO: generalize cbv*)
-Ltac debug_term_wf :=
-  let descend_wf :=
-    try(
-    eapply wf_term_by';[solve_in |  | try (left; reflexivity)];
-    let x := numgoals in
-    guard x=1;
-    (repeat (apply wf_args_cons || apply wf_args_nil));
-    debug_term_wf)
-  in
-  (compute_noconv_term_wf || descend_wf);
-  cbv - [subst_lang].
-
-
-Ltac debug_term_wf_cong_by_red :=
-  eapply wf_term_by';[solve_in |  | right; sort_cong; by_reduction];
-    let x := numgoals in
-    guard x=1;
-    (repeat (apply wf_args_cons || apply wf_args_nil));
-    cbv - [subst_lang];
-    try compute_noconv_term_wf.
-
-
-Ltac debug_gen_subst :=
-  lazymatch goal with
-    |- wf_lang_ext ((?n,term_rule ?c _ ?t)::_) _ =>
-      let mrule := eval vm_compute in
-      (substable_constr n c t)
-        in
-        lazymatch mrule with
-        | Some ?rule => push_rule_no_compute rule
-        | None => fail "Failed to generate substitution rule. TODO: improve message"
-        end
-  end.
-
 
 (* TODO: delcare interactively, register in DB *)
 Definition pi_injectivity :=
@@ -123,7 +84,6 @@ Unshelve.
 1:shelve.
 1:vm_compute; reflexivity.
 Qed.
-#[export] Hint Resolve pi_wf : elab_pfs.
+#[local] Definition pi_entry := lang_entry pi_wf.
+#[export] Hint Resolve pi_entry : wf_lang_db.
 
-#[local] Definition Pi_inst_for_db := inst_for_db "Pi".
-#[export] Hint Resolve Pi_inst_for_db : injective_con.
