src/Pyrosome/Lang/SimpleUnit.v
@@ -5,7 +5,10 @@ Import ListNotations.
 Open Scope string.
 Open Scope list.
 From Utils Require Import Utils.
-From Pyrosome Require Import Theory.Core Elab.Elab Tools.Matches Lang.SimpleVSubst Tools.EGraph.TypeInference.
+From Pyrosome Require Import Theory.Core Elab.Elab
+  Tools.Resolution Tools.EGraph.ComputeWf
+  Tools.EGraph.TypeInference.
+From Pyrosome.Lang Require Import PolySubst SimpleVSubst.
 Import Core.Notations.
 
 Definition unit_lang_def : lang :=
@@ -27,9 +30,10 @@ Definition unit_lang :=
     (infer_lang_ext_simple (exp_subst++value_subst) unit_lang_def
        (unit_injectivity++exp_subst_injectivity++value_subst_injectivity)).
 
-Lemma unit_wf : elab_lang_ext value_subst unit_lang_def unit_lang.
-Proof. auto_elab. Qed.
-#[export] Hint Resolve unit_wf : elab_pfs.
+Lemma unit_wf : wf_lang_ext value_subst unit_lang.
+Proof. compute_wf_lang. Qed.
+#[local] Definition unit_entry := lang_entry unit_wf.
+#[export] Hint Resolve unit_entry : wf_lang_db.
 
 Definition unit_eta_def :lang :=
   {[l [:= "G" : #"env",
@@ -46,6 +50,7 @@ Definition unit_eta :=
        (unit_injectivity++exp_subst_injectivity++value_subst_injectivity)).
 
 
-Lemma unit_eta_wf : elab_lang_ext (unit_lang ++ value_subst) unit_eta_def unit_eta.
-Proof. auto_elab. Qed.
-#[export] Hint Resolve unit_eta_wf : elab_pfs.
+Lemma unit_eta_wf : wf_lang_ext (unit_lang ++ value_subst) unit_eta.
+Proof. compute_wf_lang. Qed.
+#[local] Definition unit_eta_entry := lang_entry unit_eta_wf.
+#[export] Hint Resolve unit_eta_entry : wf_lang_db.
