src/Utils/Result.v
@@ -1,0 +1,18 @@
+From coqutil Require Import Datatypes.Result.
+
+(*TODO: is there a better place for this?
+  Used to put some info in the type of a failing computation.
+ *)
+Inductive Impossible {A} (a:A) : Prop := .
+Definition Is_Success {A} (r : result A) : Prop :=
+  if r then True else Impossible r.
+
+Definition true_or (b:bool) els : result unit :=
+  if b then Success tt else els.
+
+Definition Some_or {A} (b:option A) els : result A :=
+  match b with
+  | Some a => Success a
+  | None => els
+  end.
+
